theories/iris/logrel/iris_fundamental_br_table.v
@@ -16,7 +16,7 @@ Import uPred.
 Section fundamental.
   Import DummyHosts. (* placeholder *)
 
-  Context `{!wfuncG Σ, !wtabG Σ, !wtabsizeG Σ, !wmemG Σ, !wmemsizeG Σ, !wglobG Σ, !wframeG Σ, !wtablimitG Σ, !wmemlimitG Σ, HWP: host_program_logic, !logrel_na_invs Σ}.
+  Context `{!wasmG Σ, HWP: host_program_logic, !logrel_na_invs Σ}.
   
   (* --------------------------------------------------------------------------------------- *)
   (* -------------------------------------- EXPRESSIONS ------------------------------------ *)
