theories/iris/logrel/iris_fundamental_helpers.v
@@ -63,7 +63,7 @@ Qed.
 Section fundamental.
   Import DummyHosts. (* placeholder *)
 
-  Context `{!wfuncG Σ, !wtabG Σ, !wtabsizeG Σ, !wmemG Σ, !wmemsizeG Σ, !wglobG Σ, !wframeG Σ, !wtablimitG Σ, !wmemlimitG Σ, HWP: host_program_logic, !logrel_na_invs Σ}.
+  Context `{!wasmG Σ, HWP: host_program_logic, !logrel_na_invs Σ}.
   
   (* --------------------------------------------------------------------------------------- *)
   (* ------------------------------ HELPER TACTICS AND LEMMAS ------------------------------ *)
