theories/iris/rules/iris_rules_control.v
@@ -11,7 +11,7 @@ Require Export iris_wp_def stdpp_aux iris_properties.
 Close Scope byte_scope.
 Section control_rules.
   
-Context `{!wfuncG Σ, !wtabG Σ, !wtabsizeG Σ, !wtablimitG Σ, !wmemG Σ, !wmemsizeG Σ, !wmemlimitG Σ, !wglobG Σ, !wframeG Σ}.
+Context `{!wasmG Σ}.
 
 Lemma wp_br (s : stuckness) (E : coPset) (Φ : val -> iProp Σ) n vs es i LI lh f0 f:
   const_list vs ->
